backend/Renumberproof_linker.v
@@ -20,23 +20,18 @@ Set Implicit Arguments.
 
 Section PRESERVATION.
 
-Let transf_V (v_src:unit) := OK v_src.
-Let fundef_dec := (@common_fundef_dec function).
-
-Variable prog: program.
-Variable tprog: program.
+Variable (prog tprog: program).
 Hypothesis TRANSF: transf_program prog = tprog.
 
 Section FUTURE.
 
 Variable (fprog ftprog:program).
-Hypothesis (Hfsim:
-              program_weak_lsim
-                fundef_dec fn_sig fundef_dec fn_sig transf_V
-                fprog ftprog).
+Hypothesis (Hfsim: program_weak_lsim
+                     fundef_dec fn_sig fundef_dec fn_sig transf_V
+                     fprog ftprog).
 
-Hypothesis (Hfprog: program_linkeq (@common_fundef_dec function) prog fprog).
-Hypothesis (Hftprog: program_linkeq (@common_fundef_dec function) tprog ftprog).
+Hypothesis (Hfprog: program_linkeq fundef_dec prog fprog).
+Hypothesis (Hftprog: program_linkeq fundef_dec tprog ftprog).
 
 Let globfun_weak_lsim :=
   globfun_lsim fundef_dec fn_sig fundef_dec fn_sig (fun _ _ _ _ => True) fprog ftprog.
@@ -56,52 +51,30 @@ Inductive match_frames: RTL.stackframe -> RTL.stackframe -> Prop :=
       match_frames (Stackframe res f sp pc rs)
                    (Stackframe res (transf_function f) sp (renum_pc (pnum f) pc) rs).
 
-Inductive match_frames_ext (es es':list stackframe): list stackframe -> list stackframe -> Prop :=
-  | match_stackframes_ext_nil:
-      match_frames_ext es es' es es'
-  | match_stackframes_ext_cons s s' fr fr'
-      (HS: match_frames_ext es es' s s')
-      (HFR: match_frames fr fr'):
-      match_frames_ext es es' (fr::s) (fr'::s')
-.
-
-Inductive match_states (es es':list stackframe): RTL.state -> RTL.state -> Prop :=
+Inductive match_states: RTL.state -> RTL.state -> Prop :=
   | match_regular_states: forall stk f sp pc rs m stk'
-        (STACKS: match_frames_ext es es' stk stk')
+        (STACKS: list_forall2 match_frames stk stk')
         (REACH: reach f pc),
-      match_states es es'
-                   (State stk f sp pc rs m)
+      match_states (State stk f sp pc rs m)
                    (State stk' (transf_function f) sp (renum_pc (pnum f) pc) rs m)
   | match_returnstates: forall stk v m stk'
-        (STACKS: match_frames_ext es es' stk stk'),
-      match_states es es'
-                   (Returnstate stk v m)
+        (STACKS: list_forall2 match_frames stk stk'),
+      match_states (Returnstate stk v m)
                    (Returnstate stk' v m).
 
-Inductive match_call (es es':list stackframe): RTL.state -> RTL.state -> Prop :=
+Inductive match_call: RTL.state -> RTL.state -> Prop :=
   | match_callstates: forall stk f args m stk' f'
-        (STACKS: match_frames_ext es es' stk stk')
-        (FUN: fundef_weak_lsim
-                (@common_fundef_dec function) fn_sig
-                (@common_fundef_dec function) fn_sig
-                ge tge f f'),
-      match_call es es'
-                 (Callstate stk f args m)
+        (STACKS: list_forall2 match_frames stk stk')
+        (FUN: fundef_weak_lsim fundef_dec fn_sig fundef_dec fn_sig ge tge f f'),
+      match_call (Callstate stk f args m)
                  (Callstate stk' f' args m).
 
-Inductive match_return (es es':list stackframe): RTL.state -> RTL.state -> Prop :=
-  | match_return_intro: forall v m
-        (STACKS: match_frames_ext es es' es es'),
-      match_return es es'
-                   (Returnstate es v m)
-                   (Returnstate es' v m).
-
 Lemma step_simulation:
-  forall es es'  S1 t S2, RTL.step ge S1 t S2 ->
-  forall S1', match_states es es' S1 S1' -> ~ match_return es es' S1 S1' ->
-  exists S2', RTL.step tge S1' t S2' /\ (match_states es es' S2 S2' \/ match_call es es' S2 S2').
+  forall S1 t S2, RTL.step ge S1 t S2 ->
+  forall S1', match_states S1 S1' ->
+  exists S2', RTL.step tge S1' t S2' /\ (match_states S2 S2' \/ match_call S2 S2').
 Proof.
-  induction 1; intros S1' MS NMR; inv MS; try TR_AT.
+  induction 1; intros S1' MS; inv MS; try TR_AT.
 (* nop *)
   econstructor; split. eapply exec_Inop; eauto. 
   left. constructor; auto. eapply reach_succ; eauto. simpl; auto. 
@@ -164,17 +137,181 @@ Proof.
 (*     apply symbols_preserved. auto. apply varinfo_preserved. auto. *)
 (*   constructor; auto. *)
 (* return *)
-  inv STACKS; [contradict NMR; repeat (constructor; auto)|].
-  inv HFR.
+  inv STACKS. inv H1.
   econstructor; split. 
   eapply exec_return; eauto. 
   left. constructor; auto.
 Qed.
 
-(* TODO *)
+Lemma transf_initial_states:
+  forall S1, RTL.initial_state fprog S1 ->
+  exists S2, RTL.initial_state ftprog S2 /\ match_call S1 S2.
+Proof.
+  intros. inversion H. 
+  exploit funct_ptr_translated; eauto. intros [tf [A B]].
+  exists (Callstate nil tf nil m0); split.
+  econstructor; eauto.
+  eapply program_lsim_init_mem_match; eauto.
+  replace (AST.prog_main ftprog) with (AST.prog_main fprog).
+  erewrite symbols_preserved; eauto.
+  destruct Hfsim as [_ Hmain]. unfold fundef in *. rewrite <- Hmain. auto.
+  rewrite <- H3. eapply sig_preserved; eauto.
+  constructor. constructor. auto.
+Qed.
+
+Lemma transf_final_states:
+  forall S1 S2 r, match_states S1 S2 -> RTL.final_state S1 r -> RTL.final_state S2 r.
+Proof.
+  intros. inv H0. inv H. inv STACKS. constructor.
+Qed.
+
+Inductive match_states_ext st tst: Prop :=
+| match_states_ext_intro
+    (Hmatch: match_states st tst)
+    (Hsrc: ValueAnalysis_linker.sound_state_ext fprog st)
+    (Htgt: ValueAnalysis_linker.sound_state_ext ftprog tst)
+.
 
 End FUTURE.
 
-(* TODO *)
+(* memory relation *)
+
+Inductive mrelT_sem (mrel:unit) (fprog ftprog:program) (i:WF.t) (s1 s2:state): Prop :=
+| mrelT_sem_intro
+    (MEASURE: i = WF.elt)
+    (MS: match_states s1 s2 \/ match_call fprog ftprog s1 s2)
+.
+
+Definition mrelT_ops: mrelT_opsT unit :=
+  mkmrelT_opsT
+    mrelT_sem
+    (fun _ v1 v2 => v1 = v2)
+    (fun _ _ => True)
+    (fun _ _ => True).
+
+Lemma mrelT_ops_equal_list mrel v1 v2:
+  v1 = v2 <-> list_forall2 (mrelT_ops.(sem_value) mrel) v1 v2.
+Proof.
+  revert v2.
+  induction v1; intros; constructor; intro H; inv H; try constructor; simpl; auto.
+  - apply IHv1. auto.
+  - f_equal; auto. apply IHv1. auto.
+Qed.
+
+Program Definition mrelT_props: mrelT_propsT mrelT_ops := mkmrelT_propsT _ _ _ _ _ _ _.
+Next Obligation. repeat constructor. Qed.
+Next Obligation. repeat constructor. Qed.
+Next Obligation.
+  exploit transf_initial_states; eauto. intros [s2' [Hs2' Hinit]].
+  generalize (initial_state_unique Hs2' H2). intro. subst.
+  exists tt. exists WF.elt. constructor; auto.
+Qed.
+Next Obligation.
+  apply (mrelT_ops_equal_list mrel args1 args2) in Hargs.
+  inv Hs0. inv Hmrel. destruct MS as [MS|MS]; inv MS.
+
+(* external function *)
+  exists tt. exists WF.elt. eexists. eexists. eexists. split; [eauto|]. split.
+  eapply exec_function_external; eauto.
+    eapply external_call_symbols_preserved; eauto.
+    apply symbols_preserved. auto. apply varinfo_preserved. auto.
+  repeat (constructor; auto).
+Qed.
+
+Section STATE_LSIM.
+  
+Variable (fprog ftprog:program).
+Hypothesis (Hfsim: program_weak_lsim
+                     fundef_dec fn_sig fundef_dec fn_sig transf_V
+                     fprog ftprog).
+
+Hypothesis (Hfprog: program_linkeq fundef_dec prog fprog).
+Hypothesis (Hftprog: program_linkeq fundef_dec tprog ftprog).
+
+Lemma match_states_state_lsim es es' eF F i s1 s1'
+      (MS: match_states_ext fprog ftprog s1 s1'):
+  state_lsim mrelT_ops fprog ftprog es es' eF F i s1 s1'.
+Proof.
+  revert F i s1 s1' MS. pcofix CIH. intros F i s1 s1' MS. pfold.
+  inversion MS. destruct (classic (exists r, final_state s1 r)).
+  { destruct H as [rval Hrval]. eapply _state_lsim_term; eauto.
+    eapply transf_final_states; eauto.
+  }
+  constructor; auto.
+  { repeat intro. apply H. exists r0. auto. }
+  intros. exploit step_simulation; eauto. simpl.
+  intros [s2' [Hs2' Hmatch2]].
+  exists WF.elt. exists s2'. exists tt.
+  split; [destruct Hmatch2; left; apply plus_one; auto|].
+  split; auto. split; [constructor; auto|].
+  destruct Hmatch2 as [Hmatch2|Hmatch2].
+  - apply _state_lsim_or_csim_lsim. right. apply CIH.
+    constructor; auto.
+    + eapply ValueAnalysis_linker.sound_past_step; eauto.
+    + eapply ValueAnalysis_linker.sound_past_step; eauto.
+  - inversion Hmatch2. subst. eapply _state_lsim_or_csim_csim; eauto.
+    + apply (mrelT_ops_equal_list tt). auto.
+    + constructor; auto.
+    + intros. subst. inversion Hst2_mem. subst. destruct MS0 as [MS0|MS0]; [|inv MS0].
+      right. apply CIH. constructor; auto.
+Qed.
+
+Lemma transf_function_lsim f:
+  function_lsim mrelT_ops fprog ftprog f (transf_function f).
+Proof.
+  constructor. intros. pfold. constructor; subst; auto.
+  { intros ? Hfinal. inv Hfinal. }
+  intros. inversion Hst2_src. subst.
+  inv Hmrel_entry. destruct MS as [MS|MS]; inversion MS; subst.
+
+(* internal function *)
+  exists WF.elt. eexists. exists tt. split.
+  left. apply plus_one.
+  eapply exec_function_internal; eauto.
+  simpl. split; [auto|].
+  cut (match_states
+         (State cs_entry_src f (Values.Vptr stk Integers.Int.zero)
+                (fn_entrypoint f) (init_regs args_tgt (fn_params f)) m')
+         (State cs_entry_tgt (transf_function f)
+                (Values.Vptr stk Integers.Int.zero)
+                (renum_pc (postorder (successors_map f) (fn_entrypoint f))
+                          (fn_entrypoint f)) (init_regs args_tgt (fn_params f)) m')).
+  { intro MS2. split; [constructor; eauto|].
+    constructor. left. apply match_states_state_lsim. constructor; auto.
+    - eapply ValueAnalysis_linker.sound_past_step; eauto.
+    - eapply ValueAnalysis_linker.sound_past_step; eauto.
+      apply (exec_function_internal _ cs_entry_tgt (transf_function f)). auto.
+  }
+  constructor; auto. unfold reach. constructor. 
+Qed.
+
+End STATE_LSIM.
+
+Lemma Renumber_program_lsim:
+  program_lsim
+    fundef_dec fn_sig fundef_dec fn_sig transf_V
+    (function_lsim mrelT_ops)
+    prog tprog.
+Proof.
+  generalize transf_function_lsim.
+  destruct prog as [defs main]. simpl in *.
+  unfold transf_program, AST.transform_program in TRANSF.
+  inv TRANSF. intro Hlsim. constructor; simpl; auto.
+  revert Hlsim.
+  generalize defs at 1 2 3 4 as fdefs. revert defs.
+  induction defs; simpl; intros fdefs Hlsim; simpl; [constructor|].
+  destruct a. destruct g.
+  - constructor; simpl in *; try apply IHdefs; auto.
+    split; auto. constructor.
+    destruct f; simpl in *.
+    + eapply globfun_lsim_i; eauto; unfold fundef_dec, common_fundef_dec; eauto.
+      split; auto. repeat intro.
+      apply Hlsim; auto.
+    + eapply globfun_lsim_e; eauto;
+      unfold fundef_dec, common_fundef_dec; eauto.
+  - constructor; simpl in *; try apply IHdefs; auto.
+    split; auto. repeat constructor.
+    unfold AST.transf_globvar. simpl. destruct v; auto.
+Qed.
 
 End PRESERVATION.
